src/Iris/Lithium/Base.lean
@@ -1,0 +1,114 @@
+/-
+Copyright (c) 2025 Michael Sammler. All rights reserved.
+Released under Apache 2.0 license as described in the file LICENSE.
+Authors: Michael Sammler
+-/
+import Lean
+import Iris.BI
+import Iris.ProofMode
+
+namespace Iris.ProofMode
+open Lean Elab.Tactic Meta Qq BI
+
+structure PartitionHyps {prop : Q(Type u)} (bi : Q(BI $prop)) (e : Q($prop)) where
+  (espatial : Q($prop)) (hypsspatial : Hyps bi espatial)
+  (eintuit : Q($prop)) (hypsintuit : Hyps bi eintuit)
+  (pf : Q($e ⊣⊢ $espatial ∗ □ $eintuit))
+  deriving Inhabited
+
+-- TODO: use the following similar to Hyps.split?
+inductive PartitionHypsCore {prop : Q(Type u)} (bi : Q(BI $prop)) (e : Q($prop)) where
+  | none
+  | spatial
+  | intuit
+  | main (_ : PartitionHyps bi e)
+
+theorem partition_mk_emp [BI PROP] :
+    emp (PROP:=PROP) ⊣⊢ emp ∗ □ emp :=
+  sorry
+
+theorem partition_mk_intuit [BI PROP] {P : PROP} :
+    □ P ⊣⊢ emp ∗ □ □ P :=
+  sorry
+
+theorem partition_mk_spatial [BI PROP] {P : PROP} :
+    P ⊣⊢ P ∗ □ emp :=
+  sorry
+
+theorem partition_mk_merge [BI PROP] {P Ps Pi Q Qs Qi : PROP}
+  (hP : P ⊣⊢ Ps ∗ □ Pi)
+  (hQ : Q ⊣⊢ Qs ∗ □ Qi) :
+    P ∗ Q ⊣⊢ (Ps ∗ Qs) ∗ □ (Pi ∗ Qi) :=
+  sorry
+
+variable  {prop : Q(Type u)} (bi : Q(BI $prop)) in
+def Hyps.partition : ∀ {e}, Hyps bi e → PartitionHyps bi e
+  | _, .emp _ => ⟨_, .mkEmp bi, _, .mkEmp bi, q(partition_mk_emp)⟩
+  | e, h@(.hyp _ _ _ p ty _) =>
+   match matchBool p with
+   | .inl _ =>
+        have : $e =Q iprop(□ $ty) := ⟨⟩
+        ⟨_, .mkEmp bi, _, h, q(partition_mk_intuit)⟩
+   | .inr _ =>
+        ⟨_, h, _, .mkEmp bi, q(partition_mk_spatial)⟩
+  | _, .sep _ _ _ _ lhs rhs =>
+    let ⟨_, spatl, _, intuitl, pfl⟩ := lhs.partition
+    let ⟨_, spatr, _, intuitr, pfr⟩ := rhs.partition
+    ⟨_, .mkSep spatl spatr, _, .mkSep intuitl intuitr, q(partition_mk_merge $pfl $pfr)⟩
+end Iris.ProofMode
+
+
+namespace Iris.Lithium
+
+open Lean Qq Tactic Meta Iris.BI Iris.ProofMode
+
+@[match_pattern] def mkApp11 (f a b c d e₁ e₂ e₃ e₄ e₅ e₆ e₇ : Expr) := mkApp7 (mkApp4 f a b c d) e₁ e₂ e₃ e₄ e₅ e₆ e₇
+
+-- this avoids the warnings from sorry
+axiom exfalso (P : Prop) : P
+syntax "mysorry" : tactic
+macro_rules
+--| `(tactic|mysorry) => `(tactic|sorry)
+| `(tactic|mysorry) => `(tactic|apply exfalso)
+
+
+section simp
+def dsimpWithExt (ext_name : Name) (e : Expr) : MetaM (Expr × Simp.Stats) := do
+  let ext ← Lean.Meta.getSimpExtension? ext_name
+  let theorems ← ext.get!.getTheorems
+  let simpctx := ← Simp.mkContext (simpTheorems := #[theorems])
+ --let { ctx:=simpctx, .. } ← mkSimpContext .missing (eraseLocal := false) (kind := .dsimp) (simpTheorems := pure theorems)
+  -- TODO: use simpprocs as well?
+  Meta.dsimp e simpctx {}
+
+def simpWithExt (ext_name : Name) (e : Expr) (config := ({} : Simp.Config)) : MetaM (Simp.Result × Simp.Stats) := do
+  let ext ← Lean.Meta.getSimpExtension? ext_name
+  let theorems ← ext.get!.getTheorems
+  let simpctx := ← Simp.mkContext (config:=config) (simpTheorems := #[theorems])
+  Meta.simp e simpctx {}
+
+end simp
+
+
+section IrisGoalShallow
+
+structure IrisGoalShallow where
+  u : Level
+  prop : Expr
+  bi : Expr
+  hyp : Expr
+  goal : Expr
+
+def IrisGoalShallow.toExpr (g : IrisGoalShallow) : Expr :=
+  mkApp4 (.const ``Entails' [g.u]) g.prop g.bi g.hyp g.goal
+
+def parseIrisGoalShallow? (expr : Expr) : Option IrisGoalShallow := do
+  let_expr Entails' prop bi hyp goal := expr | none
+  -- dbgTrace s!"{repr (expr.getAppFn')}" λ _ =>
+  let u := expr.getAppFn'.constLevels![0]!
+  some { u, prop, bi, hyp, goal }
+
+partial def parseHypsFromShallow? (u : Level) (prop : Expr) (bi : Expr) (expr : Expr) :
+    Option ((s : Expr) × @Hyps u prop bi s) := @parseHyps? u prop bi expr
+
+end IrisGoalShallow
