src/Iris/Lithium/ExpLi.lean
@@ -1,0 +1,678 @@
+/-
+Copyright (c) 2025 Michael Sammler. All rights reserved.
+Released under Apache 2.0 license as described in the file LICENSE.
+Authors: Michael Sammler
+-/
+import Iris.BI
+import Iris.ProofMode
+import Iris.Lithium.Lithium
+import Iris.Lithium.Exp
+
+namespace Iris.ExampleLang
+open Lithium BI
+
+variable [BI.{u} PROP]
+
+section InEx
+-- TODO: Make this an atom?
+def natL (v : Val) : InEx PROP Nat := InEx.mk λ n => iprop(⌜v = .nat n⌝)
+def pairL (v : Val) : InEx PROP (Val × Val) := InEx.mk λ p => iprop(⌜v = .pair p.1 p.2⌝)
+end InEx
+
+section Li
+def expr_okR := @wp PROP _
+
+@[irun_preprocess]
+def expr_ok (e : Exp) : Li PROP Val := {
+  run := expr_okR e
+  mono' := wp_wand e
+}
+
+def app_okR (v1 v2 : Val) : (Val → PROP) → PROP := expr_okR (.app (.val v1) (.val v2))
+
+@[irun_preprocess]
+def app_ok (v1 v2 : Val) : Li PROP Val := {
+  run := app_okR v1 v2
+  mono' := wp_wand (.app (.val v1) (.val v2))
+}
+
+def recv_okR (v : Val) (E : Binder → Binder → Exp → PROP) : PROP :=
+  iprop(∃ f x e, ⌜v = .recv f x e⌝ ∗ E f x e)
+
+@[irun_preprocess]
+def recv_ok (v : Val) : Li PROP (Binder × Binder × Exp) := {
+  run E := recv_okR v λ f x e => E (f, x, e)
+  mono' E1 E2 := by mysorry
+}
+
+def subst_okR (x : Binder) (v : Val) (e : Exp) (E : Exp → PROP) : PROP :=
+  E (subst' x v e)
+
+@[irun_preprocess]
+def subst_ok (x : Binder) (v : Val) (e : Exp) : Li PROP Exp := {
+  run := subst_okR x v e
+  mono' E1 E2 := by
+    simp [subst_okR]
+    mysorry
+}
+end Li
+
+section irun
+attribute [irun_simp] Nat.add_one_sub_one
+
+@[irun]
+theorem natL_exhale_nat (n : Nat) (E : Nat → PROP) :
+  exhaleR (natL (.nat n)) E ⊣ E n := by
+  dsimp [exhaleR, natL]
+  iintro HP
+  iexists _
+  isplit
+  · ipure_intro
+    rfl
+  · iassumption
+
+@[irun]
+theorem natL_inhale_nat v :
+  inhaleR (PROP:=PROP) (natL v) :- do
+    let n ← all
+    inhale (prop (v = .nat n))
+    return n := by
+  dsimp [inhaleR, natL]
+  intro E
+  iintro HP n Hn
+  mysorry
+
+@[irun]
+theorem pairL_exhale_pair (v1 v2 : Val) (E : (Val × Val) → PROP) :
+  exhaleR (pairL (.pair v1 v2)) E ⊣ E (v1, v2) := by
+  dsimp [exhaleR, pairL]
+  iintro HP
+  iexists (_, _)
+  isplit
+  · ipure_intro
+    rfl
+  · iassumption
+
+@[irun]
+theorem pairL_inhale_pair v :
+  inhaleR (PROP:=PROP) (pairL v) :- do
+    let v1 ← all
+    let v2 ← all
+    inhale (prop (v = .pair v1 v2))
+    return (v1, v2) := by
+  dsimp [inhaleR, pairL]
+  intro E
+  iintro HP n Hn
+  mysorry
+
+@[irun]
+theorem recv_okR_rec f x e (E : Binder → Binder → Exp -> PROP) :
+  recv_okR (.recv f x e) E ⊣ E f x e := by
+  dsimp [recv_okR]
+  iintro HP
+  iexists _
+  iexists _
+  iexists _
+  isplit
+  · ipure_intro
+    rfl
+  · iassumption
+
+@[irun]
+theorem expr_okR_val v (E : Val -> PROP) :
+  expr_okR (.val v) E ⊣ E v := by mysorry
+
+@[irun]
+theorem expr_okR_plus e1 e2 :
+  expr_okR (PROP:=PROP) (Exp.binop e1 .plus e2) :- do
+   let n1 ← exhale (natL (← expr_ok e1))
+   let n2 ← exhale (natL (← expr_ok e2))
+   let n ← simp `irun_simp true (n1 + n2)
+   return (Val.nat n) := by mysorry
+
+@[irun]
+theorem expr_okR_minus e1 e2 :
+  expr_okR (PROP:=PROP) (Exp.binop e1 .minus e2) :- do
+   let n1 ← exhale (natL (← expr_ok e1))
+   let n2 ← exhale (natL (← expr_ok e2))
+   let n ← simp `irun_simp true (n1 - n2)
+   return (Val.nat n) := by mysorry
+
+@[irun]
+theorem expr_okR_eq e1 e2 :
+  expr_okR (PROP:=PROP) (Exp.binop e1 .eq e2) :- do
+   let n1 ← exhale (natL (← expr_ok e1))
+   let n2 ← exhale (natL (← expr_ok e2))
+   let n ← simp `irun_simp true (if n1 == n2 then 1 else 0)
+   return (Val.nat n)
+   := by mysorry
+
+@[irun]
+theorem expr_okR_rec f x e (E : Val -> PROP) :
+  expr_okR (.rece f x e) E ⊣ E (.recv f x e) := by mysorry
+
+@[irun]
+theorem expr_okR_let x e1 e2 :
+  expr_okR (PROP:=PROP) (.lete x e1 e2) :- do
+   let v1 ← expr_ok e1
+   let e2 ← subst_ok x v1 e2
+   let v ← expr_ok e2
+   return v
+  := by mysorry
+
+@[irun]
+theorem expr_okR_app e1 e2 :
+  expr_okR (PROP:=PROP) (.app e1 e2) :- do
+   let v2 ← expr_ok e2
+   let v1 ← expr_ok e1
+   let v ← app_ok v1 v2
+   return v
+  := by mysorry
+
+@[irun]
+theorem app_okR_recv f x e v2 :
+  app_okR (PROP:=PROP) (.recv f x e) v2 :- do
+   let v ← expr_ok (← subst_ok f (.recv f x e) (← subst_ok x v2 e))
+   return v
+  := by mysorry
+
+@[irun]
+theorem expr_okR_if e1 e2 e3 :
+  expr_okR (.ife e1 e2 e3) :- (do
+    let n1 ← exhale (natL (← expr_ok (PROP:=PROP) e1))
+    lif (n1 ≠ 0) (expr_ok e2) (expr_ok e3))
+   := by mysorry
+
+@[irun]
+theorem expr_okR_fst e :
+  expr_okR (PROP:=PROP) (.fst e) :- do
+   let v ← expr_ok e
+   let (v1, _) ← exhale (pairL v)
+   return v1 := by mysorry
+
+@[irun]
+theorem expr_okR_snd e :
+  expr_okR (PROP:=PROP) (.snd e) :- do
+   let v ← expr_ok e
+   let (_, v2) ← exhale (pairL v)
+   return v2 := by mysorry
+
+@[irun]
+theorem expr_okR_pair e1 e2 :
+  expr_okR (PROP:=PROP) (.binop e1 .pair e2) :- do
+   let v1 ← expr_ok e1
+   let v2 ← expr_ok e2
+   return (.pair v1 v2) := by mysorry
+
+end irun
+
+section subst
+open Lean Elab Tactic Meta Qq BI Std ProofMode
+
+@[irun_tac subst_okR _ _ _ _]
+def irunSubst : IRunTacticType := fun goal _config => do profileitM Exception "irunSubst" (← getOptions) do
+  let ig := goal
+  let G := ig.goal
+
+  let_expr subst_okR _ x v e E := G | return none
+  let some x := Reify.Binder.reify x | return none
+  let e := Reify.reify e
+  let e' := (Reify.subst' x v e).unreify
+  let g' := {ig with goal := Expr.beta E #[e']}.toExpr
+  let goal' ← mkFreshExprSyntheticOpaqueMVar g'
+  let pf ← mkExpectedTypeHint goal' ig.toExpr
+  return .some (pf, [goal'.mvarId!], [])
+
+end subst
+
+section fn
+
+def fn_spec (v : Val) : Atom PROP ((α : Type w) × (Val → Li PROP α) × (α → Val → Li PROP Empty)) := Atom.mk λ ⟨_, Gpre, Gpost⟩ =>
+  iprop(∀ E va,
+  (Li.bind (Gpre va) λ a =>
+   Li.bind all λ vr =>
+   Li.bind (dualizing (Gpost a vr)) λ _ =>
+   Li.pure vr).run E
+  -∗
+  wp (.app (.val v) (.val va)) E)
+
+def fn_okR {α β : Type _} (v : Val) (Gpre : Val → Li PROP α) (Gpost : α → Val → Li PROP β) (E : β → PROP) : PROP :=
+  iprop(∀ va E', (Gpre va).run E' -∗ wp (.app (.val v) (.val va)) (λ vr => iprop(∃ a, E' a ∗ (Gpost a vr).run E)))
+
+@[irun_preprocess]
+def fn_ok {α β : Type _} (v : Val) (Gpre : Val → Li PROP α) (Gpost : α → Val → Li PROP β) : Li PROP β where
+  run := fn_okR v Gpre Gpost
+  mono' E1 E2 := by mysorry
+
+theorem prove_fn_spec {α : Type _} v Gpre Gpost :
+  fn_spec (PROP:=PROP) v # ⟨α, Gpre, Gpost⟩ ⊣ (fn_ok v Gpre Gpost).go := by
+  mysorry
+
+@[irun]
+theorem fn_okR_recv α β f x e Gpre Gpost E :
+  @fn_okR PROP _ α β (.recv f x e) Gpre Gpost E ⊣
+   allR λ va =>
+   allR λ v' =>
+   allR λ Φ : Atom PROP α =>
+   inhaleR (pers (atom_with_ref (fn_spec v') ⟨α, Gpre, λ a vr => (Gpost a vr).bind λ _ => done⟩)) λ _ =>
+   ((Gpre va).run) |> λ Gpre' =>
+   dualizingR (λ _ => Gpre' λ a => exhaleR (atom_with_ref Φ a) λ _ => doneR) λ _ =>
+   subst_okR x va e λ e =>
+   subst_okR f v' e λ e =>
+   expr_okR e λ vr =>
+   exhaleR (atom Φ) λ a =>
+   ((Gpost a vr).run) |> λ Gpost =>
+   Gpost E := by mysorry
+
+@[irun:mid] -- This should be tried after the .recv version
+theorem fn_okR_subsume (α β : Type _) v Gpre Gpost E :
+  @fn_okR PROP _ α β v Gpre Gpost E ⊣
+   exhaleR (atom (fn_spec v)) λ ⟨_, Gpre2, Gpost2⟩ =>
+   allR λ va =>
+   allR λ Φpre : Atom PROP α =>
+   dualizingR (λ _ => (Gpre va).run λ a => exhaleR (atom_with_ref Φpre a) λ _ => doneR) λ _ =>
+   (Gpre2 va).run λ c =>
+   exhaleR (atom Φpre) λ a =>
+   allR λ vr =>
+   dualizingR ((Gpost2 c vr).run) λ _ =>
+   (Gpost a vr).run E
+    := by mysorry
+
+-- should be applied after the inlining rule
+@[irun:low]
+theorem app_okR_spec v1 v2 :
+  app_okR (PROP:=PROP) v1 v2 :-
+   (exhale (atom (fn_spec v1))).bind λ ⟨_, Gpre, Gpost⟩ =>
+   (Gpre v2).bind λ a =>
+   all.bind λ vr =>
+   (dualizing (Gpost a vr)).bind λ _ =>
+   Li.pure vr
+  := by mysorry
+
+@[irun]
+theorem dualizing_fn_ok α β E v Gpre Gpost (G : _ → _) :
+  dualizingR (PROP:=PROP) (λ E => @fn_okR PROP _ α β v Gpre Gpost (G E)) E ⊣
+    inhaleR (atom_with_ref (fn_spec v) ⟨_, Gpre, λ a vr => (Gpost a vr).bind λ b => fromEmpty (λ E => G E b)⟩) E
+ := by mysorry
+
+-- TODO: Allow G E instead of just E in the continuation for fn_okR?
+@[irun]
+theorem inhale_persLi_fn_ok α β E v Gpre Gpost (hmono : ∀ _ _, ⊢ _) :
+  inhaleR (PROP:=PROP)
+    (persLi (Li.mk (λ E => @fn_okR PROP _ α β v Gpre Gpost E) hmono)) E ⊣
+    inhaleR (pers (atom_with_ref (fn_spec v) ⟨_, Gpre, λ a vr => (Gpost a vr).bind λ _ => done⟩)) E
+ := by mysorry
+end fn
+
+section ptsto
+def ptsto (v : Val) : Atom PROP Val := sorry
+
+@[irun]
+theorem expr_okR_alloc :
+  expr_okR (PROP:=PROP) .alloc :- do
+    let v ← all
+    inhale (atom_with_ref (ptsto v) (.nat 0))
+    return v := by mysorry
+
+@[irun]
+theorem expr_okR_store e1 e2 :
+  expr_okR (PROP:=PROP) (.store e1 e2) :- do
+    let v2 ← expr_ok e2
+    let v1 ← expr_ok e1
+    let _ ← exhale (atom (ptsto v1))
+    inhale (atom_with_ref (ptsto v1) v2)
+    return v2 := by mysorry
+
+@[irun]
+theorem expr_okR_load e :
+  expr_okR (PROP:=PROP) (.load e) :- do
+    let v ← expr_ok e
+    let vl ← exhale (atom (ptsto v))
+    inhale (atom_with_ref (ptsto v) vl)
+    return vl := by mysorry
+end ptsto
+
+section test
+example (P : Val -> Atom PROP Unit) :
+  ⊢ (do
+      inhale (atom_with_ref (P (.nat 10)) ())
+      let v ← expr_ok (.binop (.val (.nat 5)) .plus (.val (.nat 5)))
+      exhale (atom (P v))
+      done).go := by
+  istart
+  simp only [irun_preprocess]
+  irun
+
+-- time: ~1700ms (when using trivial for irun_solve)
+-- time: ~2559ms (when using simp for irun_solve)
+-- time: ~3190ms (when using simp for irun_solve after updating to 4.19.0?)
+-- set_option profiler true in
+--set_option profiler.threshold 1 in
+set_option Elab.async false in
+--set_option trace.profiler true in
+--set_option trace.profiler.threshold 5 in
+--set_option trace.IRun.step true in
+#time example (P : Val -> Atom PROP Unit) :
+   ⊢ (do
+        inhale (atom_with_ref (P (.nat 0)) ())
+        let v ← expr_ok (.app (.val rec_fn) (.val (.nat 200)))
+        exhale (atom (P v))
+        done).go := by
+  istart
+  unfold rec_fn
+  simp only [irun_preprocess]
+  --set_option trace.profiler true in
+  --set_option trace.profiler.threshold 1 in
+  --set_option diagnostics true in
+  --set_option profiler true in
+  irun ∞
+
+
+example :
+  ⊢ fn_spec (PROP:=PROP) rec_fn # ⟨Nat, λ va => exhale (natL va), λ _ _ => done⟩ := by
+  unfold rec_fn
+  apply (BI.BIBase.Entails.trans _ (prove_fn_spec _ _ _))
+  istart
+  simp only [irun_preprocess]
+  irun
+
+end test
+
+section echo
+def getc_fn : Val := .recv .anon .anon (.val (.nat 1))
+def putc_fn : Val := .recv .anon .anon (.val (.nat 1))
+def echo_fn : Val := .recv .anon .anon (.lete "x" (.app (.val getc_fn) (.val (.nat 0))) (.app (.val putc_fn) (.var "x")))
+def main_fn : Val := .recv .anon .anon (.app (.val echo_fn) (.val (.nat 0)))
+
+def echo_spec PROP [BI PROP] : PROP :=
+  fn_spec echo_fn # ⟨_,
+     λ _ => do
+      fn_ok getc_fn
+        (λ _ => .pure ())
+         λ _ vr => do
+      fn_ok putc_fn
+        (λ va => exhale (prop (va = vr)))
+         λ _ vrp => .pure vrp,
+     λ vrp vr => do exhale (prop (vrp = vr)); done ⟩
+
+theorem echo_ok :
+  ⊢ echo_spec PROP := by
+  unfold echo_spec echo_fn
+  apply (BI.BIBase.Entails.trans _ (prove_fn_spec _ _ _))
+  istart
+  simp only [irun_preprocess]
+  irun
+
+theorem main_ok [BIAffine PROP] :
+  echo_spec PROP ⊢ (fn_spec main_fn) # ⟨_, λ _ => .pure (), λ _ vr => do exhale (prop (vr = .nat 1)); done⟩ := by
+  unfold echo_spec main_fn getc_fn putc_fn
+  apply (BI.BIBase.Entails.trans _ (prove_fn_spec _ _ _))
+  istart
+  iintro x
+  simp only [irun_preprocess]
+  irun
+
+end echo
+
+section fib
+def fib_fn : Val := .recv "f" "x" <|
+  .ife (.binop (.var "x") .eq (.val (.nat 0)))
+    (.val (.nat 0)) <|
+  .ife (.binop (.var "x") .eq (.val (.nat 1)))
+    (.val (.nat 1)) <|
+   .binop (.app (.var "f") (.binop (.var "x") .minus (.val (.nat 1)))) .plus
+     (.app (.var "f") (.binop (.var "x") .minus (.val (.nat 2))))
+
+@[irun_solve]
+def fib : Nat → Nat
+  | 0 => 0
+  | 1 => 1
+  | n+1+1 => fib n + fib (n + 1)
+
+theorem fib_ok [BIAffine PROP] :
+  ⊢ (fn_spec (PROP:=PROP) fib_fn) # ⟨_,
+    λ va => do {let n ← exhale (natL va); exhale (prop (0 ≤ n)); return n},
+    λ n vr => do {let nr ← exhale (natL vr); exhale (prop (nr = fib n)); done}⟩ := by
+  unfold fib_fn
+  apply (BI.BIBase.Entails.trans _ (prove_fn_spec _ _ _))
+  istart
+  simp only [irun_preprocess]
+  irun
+  · rename Nat => x
+    cases x using fib.fun_cases <;> simp [fib] at * <;> omega
+
+end fib
+
+section ptsto
+def ptsto_test : Exp :=
+  .lete "l" (.alloc) <|
+  .lete .anon (.store (.var "l") (.load (.var "l"))) <|
+  .var "l"
+
+example :
+  ⊢ (do
+    let v ← expr_ok (PROP:=PROP) ptsto_test
+    let vl ← exhale (atom (ptsto v) >>= natL)
+    exhale (prop (0 ≤ vl))
+    done).go := by
+  istart
+  simp [irun_preprocess, ptsto_test]
+  irun
+end ptsto
+
+section tutorial
+def NULL : Val := .nat 0
+
+def is_list (v : Val) : Atom PROP (List Val) := sorry
+
+@[irun]
+theorem exhaleR_is_list_NULL :
+  exhaleR (PROP:=PROP) (atom (is_list NULL)) :- return [] := by mysorry
+
+@[irun]
+theorem cancel_ptsto_list v x :
+  cancelR (PROP:=PROP) (ptsto v # x) (is_list v) :- do
+    let (v1, v2) ← exhale (pairL x)
+    let xs ← exhale (atom (is_list v2))
+    return v1 :: xs := by mysorry
+
+@[irun]
+theorem cancel_list_ptsto v xs :
+  cancelR (PROP:=PROP) (is_list v # xs) (ptsto v) :- do
+    exhale (prop (0 < xs.length))
+    let v' ← all
+    let x ← all
+    let xs' ← inhale (atom (is_list v'))
+    inhale (prop (xs = x::xs'))
+    return .pair x v' := by mysorry
+
+
+def is_null (v : Val) : Atom PROP Bool := sorry
+
+-- TODO: handle this with binop ok to allow proper overloading
+@[irun:high]
+theorem expr_okR_eq_NULL e1 :
+  expr_okR (PROP:=PROP) (Exp.binop e1 .eq (.val NULL)) :- do
+   let b ← exhale (atom (is_null (← expr_ok e1)))
+   return (Val.nat (if b then 1 else 0))
+   := by mysorry
+
+@[irun]
+theorem cancel_is_null_ptsto v v' :
+  cancelR (PROP:=PROP) (ptsto v # v') (is_null v) :- do
+    inhale (atom_with_ref (ptsto v) v')
+    return false := by mysorry
+
+@[irun]
+theorem cancel_is_null_list v xs :
+  cancelR (PROP:=PROP) (is_list v # xs) (is_null v) :- do
+    inhale (atom_with_ref (is_list v) xs)
+    return xs.isEmpty := by mysorry
+
+
+def empty_fn : Val := .recv .anon .anon (.val NULL)
+def cons_fn : Val := .recv .anon "a" <|
+  .lete "v" (.fst (.var "a")) <|
+  .lete "l" (.snd (.var "a")) <|
+  .lete "new_l" (.alloc) <|
+  .lete .anon (.store (.var "new_l") (.binop (.var "v") .pair (.var "l"))) <|
+  .var "new_l"
+
+def mklist_fn : Val := .recv .anon .anon <|
+  .lete "l" (.app (.val empty_fn) (.val (.nat 0))) <|
+  .lete "l" (.app (.val cons_fn) (.binop (.val (.nat 1)) .pair (.var "l"))) <|
+  .lete "l" (.app (.val cons_fn) (.binop (.val (.nat 2)) .pair (.var "l"))) <|
+  .var "l"
+
+theorem empty_ok [BIAffine PROP] :
+  ⊢ fn_spec (PROP:=PROP) empty_fn # ⟨_,
+    λ _ => do {return ()},
+    λ _ vr => do {let vs ← exhale (atom (is_list vr)); exhale (prop (vs = [])); done}⟩ := by
+  unfold empty_fn
+  apply (BI.BIBase.Entails.trans _ (prove_fn_spec _ _ _))
+  istart
+  simp only [irun_preprocess]
+  irun
+
+theorem cons_ok [BIAffine PROP] :
+  ⊢ (fn_spec (PROP:=PROP) cons_fn) # ⟨_,
+    λ va => do {let (x, v) ← exhale (pairL va); let xs ← exhale (atom (is_list v)); return (x, xs)},
+    λ (x, xs) vr => do {let vs ← exhale (atom (is_list vr)); exhale (prop (vs = x::xs)); done}⟩ := by
+  unfold cons_fn
+  apply (BI.BIBase.Entails.trans _ (prove_fn_spec _ _ _))
+  istart
+  simp only [irun_preprocess]
+  irun
+
+theorem mklist_ok [BIAffine PROP] :
+  □ fn_spec (PROP:=PROP) empty_fn # ⟨_,
+    λ _ => do {return ()},
+    λ _ vr => do {let vs ← exhale (atom (is_list vr)); exhale (prop (vs = [])); done}⟩ ∗
+  □ fn_spec (PROP:=PROP) cons_fn # ⟨_,
+    λ va => do {let (x, v) ← exhale (pairL va); let xs ← exhale (atom (is_list v)); return (x, xs)},
+    λ (x, xs) vr => do {let vs ← exhale (atom (is_list vr)); exhale (prop (vs = x::xs)); done}⟩
+  ⊢ fn_spec (PROP:=PROP) mklist_fn # ⟨_,
+    λ _ => do {return ()},
+    λ _ vr => do {let vs ← exhale (atom (is_list vr)); exhale (prop (vs = [.nat 2, .nat 1])); done}⟩ := by
+  unfold mklist_fn
+  apply (BI.BIBase.Entails.trans _ (prove_fn_spec _ _ _))
+  istart
+  iintro ⟨□ h1, □ h2⟩
+  simp only [irun_preprocess]
+  irun
+
+
+def head_fn : Val := .recv .anon "l" (.fst (.load (.var "l")))
+
+theorem head_ok :
+  ⊢ fn_spec (PROP:=PROP) head_fn # ⟨_,
+    λ va => do {let xs ← exhale (atom (is_list va)); exhale (prop (0 < xs.length)); return (va, xs)},
+    λ (va, xs) vr => do {exhale (atom_with_ref (is_list va) xs); exhale (prop (xs.head? = some vr)); done}⟩ := by
+  unfold head_fn
+  apply (BI.BIBase.Entails.trans _ (prove_fn_spec _ _ _))
+  istart
+  simp only [irun_preprocess]
+  irun
+
+def length_fn : Val := .recv "f" "l" <|
+  .ife (.binop (.var "l") .eq (.val NULL))
+    (.val (.nat 0)) <|
+  .lete "r" (.app (.var "f") (.snd (.load (.var "l")))) <|
+  .binop (.var "r") .plus (.val (.nat 1))
+
+theorem length_ok :
+  ⊢ fn_spec (PROP:=PROP) length_fn # ⟨_,
+    λ va => do {let xs ← exhale (atom (is_list va)); return (va, xs)},
+    λ (va, xs) vr => do {exhale (atom_with_ref (is_list va) xs); exhale (prop (vr = .nat xs.length)); done}⟩ := by
+  unfold length_fn
+  apply (BI.BIBase.Entails.trans _ (prove_fn_spec _ _ _))
+  istart
+  simp only [irun_preprocess]
+  irun
+  rename List Val => xs
+  cases xs <;> simp at *
+
+def contains_fn : Val := .recv "f" "x" <|
+  .lete "l" (.fst (.var "x")) <|
+  .lete "cb" (.snd (.var "x")) <|
+  .ife (.binop (.var "l") .eq (.val NULL))
+    (.val (.nat 0)) <|
+  .ife (.app (.var "cb") (.fst (.load (.var "l"))))
+    (.val (.nat 1)) <|
+  .app (.var "f") (.binop (.snd (.load (.var "l"))) .pair (.var "cb"))
+
+def contains_spec_pre (P : Val → Bool) : Val → Li PROP (Val × List Val) :=
+    λ v => do
+      let (va, cb) ← exhale (pairL v)
+      let xs ← exhale (atom (is_list va))
+      exhale (persLi (fn_ok cb
+        (λ va => do {exhale (prop (va ∈ xs)); return va})
+        (λ va vr => do {exhale (prop (vr = .nat (if P va then 1 else 0))); return ()})))
+      return (va, xs)
+
+def contains_spec_post (P : Val → Bool) : (Val × List Val) → Val → Li PROP Empty :=
+  λ (va, xs) vr => do
+      exhale (atom_with_ref (is_list va) xs)
+      exhale (prop (vr = .nat (if xs.any P then 1 else 0)))
+      done
+
+def contains_spec (P : Val → Bool) : PROP :=
+  fn_spec (PROP:=PROP) contains_fn # ⟨_, contains_spec_pre P, contains_spec_post P⟩
+
+
+set_option Elab.async false in
+--set_option trace.profiler true in
+--set_option trace.IRun.step true in
+--set_option trace.profiler.threshold 5 in
+-- time: ~578ms
+#time theorem contains_ok [BIAffine PROP] P :
+  ⊢ contains_spec (PROP:=PROP) P := by
+  unfold contains_spec contains_spec_pre contains_spec_post contains_fn
+  apply (BI.BIBase.Entails.trans _ (prove_fn_spec _ _ _))
+  istart
+  simp only [irun_preprocess]
+  irun
+  rename List Val => xs
+  cases xs <;> simp at *
+
+def contains_one_fn : Val := .recv .anon "x" <|
+  .app (.val contains_fn) (.binop (.var "x") .pair (.rece .anon "y" <| .binop (.var "y") .eq (.val (.nat 1))))
+
+-- TODO: profile this, this is slower than the Rocq version
+-- TODO: The profile says "tactic execution of Lean.Parser.Tactic.refine took 654ms". Where does this come from?
+set_option Elab.async false in
+--set_option trace.profiler true in
+--set_option trace.profiler.threshold 10 in
+--set_option trace.IRun.step true in
+--set_option profiler true in
+-- time: 261ms
+#time theorem contains_one_ok [BIAffine PROP] :
+  ⊢ (do
+    inhale (pers (atom_with_ref (fn_spec contains_fn)
+      ⟨_, contains_spec_pre (λ v => v == Val.nat 1), contains_spec_post (λ v => v == Val.nat 1)⟩))
+    fn_ok (PROP:=PROP) contains_one_fn
+      (λ va => do
+        let xs ← exhale (atom (is_list va))
+        exhale (prop (∀ x ∈ xs, ∃ n, x = Val.nat n))
+        return (va, xs))
+      (λ (va, xs) vr => do
+        exhale (atom_with_ref (is_list va) xs)
+        exhale (prop (vr = Val.nat (if Val.nat 1 ∈ xs then 1 else 0)))
+        done)).go := by
+  unfold contains_spec_pre contains_spec_post contains_one_fn
+  istart
+
+  -- Time goes from ~300ms to ~2000ms if one removes the only. Why?
+  simp only [irun_preprocess]
+  -- iintro □h
+  irun
+--  all_goals mysorry
+  -- TODO: automate this somehow?
+  rename_i v v2 Φ Hin
+  have ⟨n, Hn⟩ : ∃ n, v = .nat n := by simp [*]
+  simp only [Hn]
+  irun
+
+end tutorial
+
+end Iris.ExampleLang
