src/Iris/Lithium/IRunAttr.lean
@@ -3,52 +3,16 @@ Copyright (c) 2025 Michael Sammler. All rights reserved.
 Released under Apache 2.0 license as described in the file LICENSE.
 Authors: Michael Sammler
 -/
-import Lean
-import Qq
 import Iris.BI
 import Iris.ProofMode
+import Iris.Lithium.Base
 
-open Lean Elab Tactic Meta Qq Iris.BI
-
-namespace Iris.ProofMode
-
-def dsimpWithExt (ext_name : Name) (e : Expr) : MetaM (Expr × Simp.Stats) := do
-  let ext ← Lean.Meta.getSimpExtension? ext_name
-  let theorems ← ext.get!.getTheorems
-  let simpctx := ← Simp.mkContext (simpTheorems := #[theorems])
- --let { ctx:=simpctx, .. } ← mkSimpContext .missing (eraseLocal := false) (kind := .dsimp) (simpTheorems := pure theorems)
-  -- TODO: use simpprocs as well?
-  Meta.dsimp e simpctx {}
-
-def simpWithExt (ext_name : Name) (e : Expr) (config := ({} : Simp.Config)) : MetaM (Simp.Result × Simp.Stats) := do
-  let ext ← Lean.Meta.getSimpExtension? ext_name
-  let theorems ← ext.get!.getTheorems
-  let simpctx := ← Simp.mkContext (config:=config) (simpTheorems := #[theorems])
-  Meta.simp e simpctx {}
+namespace Iris.Lithium
+open Lean Elab Tactic Meta Iris.BI Iris.ProofMode
 
 register_simp_attr irun_simp
 register_simp_attr irun_solve
 register_simp_attr irun_preprocess
-
-structure IrisGoalShallow where
-  u : Level
-  prop : Expr
-  bi : Expr
-  hyp : Expr
-  goal : Expr
-
-def IrisGoalShallow.toExpr (g : IrisGoalShallow) : Expr :=
-  mkApp4 (.const ``Entails' [g.u]) g.prop g.bi g.hyp g.goal
-
-def parseIrisGoalShallow? (expr : Expr) : Option IrisGoalShallow := do
-  let_expr Entails' prop bi hyp goal := expr | none
-  -- dbgTrace s!"{repr (expr.getAppFn')}" λ _ =>
-  let u := expr.getAppFn'.constLevels![0]!
-  some { u, prop, bi, hyp, goal }
-
-partial def parseHypsFromShallow? (u : Level) (prop : Expr) (bi : Expr) (expr : Expr) :
-    Option ((s : Expr) × @Hyps u prop bi s) := @parseHyps? u prop bi expr
-
 
 structure IRunConfig where
   debug := false
@@ -56,9 +20,11 @@ structure IRunConfig where
 
 declare_config_elab elabIRunConfig IRunConfig
 
+
 def IRunTacticType : Type := IrisGoalShallow → IRunConfig → TacticM (Option (Expr × List MVarId × List MVarId))
 
 def IRunTacticType.run (tac : IRunTacticType) : IrisGoalShallow → IRunConfig → TacticM (Option (Expr × List MVarId × List MVarId)) := tac
+
 
 structure IRunTactic where
   tac : IRunTacticType
@@ -98,22 +64,23 @@ def IRunEntry.serialize (e : IRunEntry) : IRunEntrySerialized := {
 def IRunEntrySerialized.deserialize (e : IRunEntrySerialized) (compile : Bool) : CoreM IRunEntry := do
   -- IO.println s!"deserializing {repr e}"
   let tac  ← match e.tac with
-           | .inl n => .pure (.inl n)
-           | .inr n => unsafe do
-             let ty := (← getConstInfo n.name).type
-             if ty != .const ``IRunTacticType [] then
-               throwError "The tactic should have type IRunTacticType."
-             if compile then
-               -- is this the compilation the right thing to do?
-               let .defnInfo d ← getConstInfo n.name | throwError "The tactic should be a definition."
-               let decl := (.defnDecl d)
-               try
-                 withOptions (λ opt => Elab.async.set opt false) <|
-                   compileDecl decl
-               catch e =>
-                 IO.println (s!"error while compiling {n.name}: {← e.toMessageData.toString}")
-             let tac ← evalConst IRunTacticType n.name
-             return (.inr ⟨tac, n.name⟩ : Name ⊕ IRunTactic)
+    | .inl n => .pure (.inl n)
+    | .inr n => unsafe do
+      let ty := (← getConstInfo n.name).type
+      if ty != .const ``IRunTacticType [] then
+        throwError "The tactic should have type IRunTacticType."
+      if compile then
+        -- is this the compilation the right thing to do?
+        let .defnInfo d ← getConstInfo n.name |
+          throwError "The tactic should be a definition."
+        let decl := (.defnDecl d)
+        try
+          withOptions (λ opt => Elab.async.set opt false) <|
+            compileDecl decl
+        catch e =>
+          IO.println s!"error while compiling {n.name}: {← e.toMessageData.toString}"
+      let tac ← evalConst IRunTacticType n.name
+      return (.inr ⟨tac, n.name⟩ : Name ⊕ IRunTactic)
   return {tac, prio := e.prio, name := e.name}
 
 /-- Environment extension for `irun` -/
@@ -166,8 +133,7 @@ initialize registerBuiltinAttribute {
 
 syntax (name := irun_tac) "irun_tac" (":" prio)? (ppSpace term),* : attr
 
--- TODO: Is this unsafe a problem? Can we get around it?
-initialize unsafe registerBuiltinAttribute {
+initialize registerBuiltinAttribute {
   name := `irun_tac
   descr := "irun tactic"
   -- we ignore TC failures for BI, they should just create metavariables
