src/Iris/Lithium/Lithium.lean
@@ -1,0 +1,697 @@
+/-
+Copyright (c) 2025 Michael Sammler. All rights reserved.
+Released under Apache 2.0 license as described in the file LICENSE.
+Authors: Michael Sammler
+-/
+import Iris.BI
+import Iris.ProofMode
+import Iris.Lithium.IRunAttr
+import Iris.Lithium.IRun
+
+namespace Iris.Lithium
+open Lean Elab.Tactic Meta Qq BI
+
+attribute [irun_preprocess] Pure.pure Bind.bind
+
+-- TODO: use something shorter than PROP? E.g. ℙ (\bbP) or Ω?
+variable {PROP : Type u} [BI.{u} PROP] {α : Type v} {β : Type w}
+
+structure Atom (PROP : Type u) (α : Type v) where
+  ref : α → PROP
+
+-- TODO: Better symbol?
+-- TODO: What are good precedences here?
+notation:90 A:90 " # " a:90 => (Atom.ref A a)
+delab_rule Atom.ref
+  | `($_ $A $a) => do ``($A # $a)
+
+structure InEx (PROP : Type u) (α : Type v) where
+  body : α → PROP
+
+structure Li (PROP : Type u) [BI.{u} PROP] (α : Type v) where
+  run : (α → PROP) → PROP
+  mono' E1 E2 : ⊢ run E1 -∗ (∀ a, E1 a -∗ E2 a) -∗ run E2
+
+-- This prevents printing mono := ...
+-- TODO: Is this a good idea?
+delab_rule Li.mk
+  | `($_ $run $_) => do ``($run)
+
+section InEx
+
+def InEx.pure (a : α) : InEx PROP α :=
+  InEx.mk λ b => iprop(⌜a = b⌝)
+
+def InEx.bind (L1 : InEx PROP α) (L2 : α → InEx PROP β) :
+  InEx PROP β :=
+  InEx.mk λ b => iprop(∃ a, L1.body a ∗ (L2 a).body b)
+
+instance : Monad (InEx PROP) where
+  pure := .pure
+  bind := .bind
+
+-- TODO: Use this and add it for Li
+instance : HAndThen (InEx PROP α) (InEx PROP β) (InEx PROP β) where
+  hAndThen L1 L2 := L1.bind λ _ => L2 ()
+
+def atom (A : Atom PROP α) : InEx PROP α := InEx.mk A.ref
+def atom_with_ref (A : Atom PROP α) (a : α) : InEx PROP Unit := .mk λ _ => iprop(A # a)
+def prop (P : Prop) : InEx PROP Unit := .mk λ _ => iprop(⌜P⌝)
+def pers (L : InEx PROP α) : InEx PROP α := .mk λ a => iprop(□ L.body a)
+def persLi (G : Li PROP α) : InEx PROP Unit := .mk λ _ => iprop(□ G.run λ _ => iprop(True))
+
+end InEx
+
+section Li
+@[irun_preprocess]
+def Li.pure (a : α) : Li PROP α := {
+  run E := E a
+  mono' E1 E2 := by
+    iintro HE Hwand
+    ispecialize Hwand HE
+    iassumption
+}
+
+@[irun_preprocess]
+def Li.bind (G1 : Li PROP α) (G2 : α → Li PROP β) :
+  Li PROP β := {
+  run E := G1.run (λ a => (G2 a).run E)
+  mono' E1 E2 := by
+    iintro HE Hwand
+    mysorry
+}
+
+instance : Monad (Li PROP) where
+  pure := .pure
+  bind := .bind
+
+def empty : Empty → PROP := λ e => nomatch e
+
+@[irun_preprocess]
+def Li.go (G : Li PROP Empty) : PROP := G.run empty
+
+def exhaleR (L : InEx PROP α) (E : α → PROP) : PROP :=
+  iprop(∃ a, L.body a ∗ E a)
+
+@[irun_preprocess]
+def exhale (L : InEx PROP α) : Li PROP α := {
+  run := exhaleR L
+  mono' E1 E2 := by
+    dsimp [exhaleR]
+    iintro ⟨a, HL, HE⟩ Hwand
+    iexists a
+    isplit l [HL]
+    iassumption
+    ispecialize Hwand HE
+    iassumption
+}
+
+def inhaleR (L : InEx PROP α) (E : α → PROP) : PROP :=
+  iprop(∀ a, L.body a -∗ E a)
+
+@[irun_preprocess]
+def inhale (L : InEx PROP α) : Li PROP α := {
+  run := inhaleR L
+  mono' E1 E2 := by
+    dsimp [inhaleR]
+    iintro HE Hwand a HL
+    ispecialize HE HL
+    ispecialize Hwand HE
+    iassumption
+}
+
+def cancelR (P : PROP) (A : Atom PROP α) (E : α → PROP) : PROP :=
+  iprop(P -∗ ∃ a, A # a ∗ E a)
+
+@[irun_preprocess]
+def cancel (P : PROP) (A : Atom PROP α) : Li PROP α := {
+  run := cancelR P A
+  mono' E1 E2 := by
+    dsimp [cancelR]
+    mysorry
+}
+
+def allR {α : Type v} (E : α → PROP) : PROP :=
+  iprop(∀ a, E a)
+
+@[irun_preprocess]
+def all {α : Type v} : Li PROP α := {
+  run := @allR _ _ α
+  mono' E1 E2 := by
+    dsimp [allR]
+    iintro HE Hwand a
+    ispecialize HE a
+    ispecialize Hwand HE
+    iassumption
+}
+
+def doneR : PROP := iprop(True)
+
+@[irun_preprocess]
+def done : Li PROP α := {
+  run E := doneR
+  mono' E1 E2 := by
+    dsimp [doneR]
+    iintro HE Hwand
+    iassumption
+}
+
+def branchR (E1 E2 : PROP) : PROP :=
+  iprop(E1 ∧ E2)
+
+@[irun_preprocess]
+def branch (G1 G2 : Li PROP α) : Li PROP α := {
+  run E := branchR (G1.run E) (G2.run E)
+  mono' E1 E2 := by
+    iintro HE Hwand
+    mysorry
+}
+
+def lifR (P : Prop) (E1 E2 : PROP) : PROP :=
+  iprop((⌜P⌝ -∗ E1) ∧ (⌜¬P⌝ -∗ E2))
+
+@[irun_preprocess]
+def lif (P : Prop) (G1 G2 : Li PROP α) : Li PROP α := {
+  run E := lifR P (G1.run E) (G2.run E)
+  mono' E1 E2 := by
+    iintro HE Hwand
+    mysorry
+}
+
+def dropSpatialR (G : PROP) : PROP :=
+  iprop(□ G)
+
+@[irun_preprocess]
+def dropSpatial (G : Li PROP α) : Li PROP α := {
+  run E := dropSpatialR (G.run E)
+  mono' E1 E2 := by
+    iintro HE Hwand
+    mysorry
+}
+
+def simpR {α : Type _} [BI PROP] (_ : Lean.Name) (_dsimp : Bool) (a : α) (E : α → PROP) : PROP := E a
+
+@[irun_preprocess]
+def simp {α : Type _} [BI PROP] (n : Lean.Name) (dsimp : Bool) (a : α) : Li PROP α := {
+  run := simpR n dsimp a
+  mono' E1 E2 := by
+    simp [simpR]
+    mysorry
+}
+
+def dualizingR (G : (Empty → PROP) → PROP) (E : Unit → PROP) : PROP :=
+  iprop(G empty -∗ E ⟨⟩)
+
+@[irun_preprocess]
+def dualizing (G : Li PROP Empty) : Li PROP Unit := {
+  run := dualizingR G.run
+  mono' E1 E2 := by
+    dsimp [dualizingR]
+    iintro HE Hwand HG
+    ispecialize HE HG
+    ispecialize Hwand HE
+    iassumption
+}
+
+@[irun_preprocess]
+def fromEmpty (G : (Empty → PROP) → PROP) : Li PROP Empty where
+  run := G
+  mono' E1 E2 := by
+   have HE : (E1 = E2) := by ext x; nomatch x
+   simp [HE]
+   mysorry
+
+end Li
+
+def test_lithium (A : Atom PROP Nat) : Li PROP Bool := do
+  let b ← exhale do
+    let n ← atom A
+    return (n == 1)
+  inhale do
+    let n ← atom A
+    prop (b = (n == 1))
+    return true
+
+notation:25 P:29 "⊣" Q:25 => (Q ⊢ P)
+set_option quotPrecheck false in -- TODO: Why is this necessary?
+notation:25 P:29 ":-" Q:25 => (∀ E, Li.run Q E ⊢ P E)
+
+section irun
+@[irun]
+theorem exhale_bind (L1 : InEx PROP α) (L2 : α → InEx PROP β) :
+  exhaleR (L1.bind L2) :-
+    ((exhale L1).bind λ a => exhale (L2 a)) := by
+    dsimp [exhaleR, InEx.bind]
+    mysorry
+
+@[irun]
+theorem inhale_bind (L1 : InEx PROP α) (L2 : α → InEx PROP β) E :
+  inhaleR (L1.bind L2) E ⊣
+   inhaleR L1 λ a => inhaleR (L2 a) E := by
+    dsimp [inhaleR, InEx.bind]
+    mysorry
+
+@[irun]
+theorem exhale_pure (a : α) E :
+  exhaleR (PROP:=PROP) (.pure a) E ⊣ E a := by
+    dsimp [exhaleR, InEx.pure]
+    mysorry
+
+@[irun]
+theorem inhale_pure (a : α) E :
+  inhaleR (PROP:=PROP) (.pure a) E ⊣ E a := by
+    dsimp [inhaleR, InEx.pure]
+    mysorry
+
+end irun
+
+end Iris.Lithium
+
+namespace Iris.Lithium
+open Lean Elab Tactic Meta Qq BI Std Lithium ProofMode
+
+section inhale
+
+@[irun]
+theorem inhale_atom [BI PROP] {α : Type _} A (E : α → PROP) :
+   inhaleR (atom A) E ⊣ allR λ a => inhaleR (atom_with_ref A a) λ _ => E a :=
+   by mysorry
+
+
+theorem inhale_atom_with_ref_tac {α : Type _} [BI PROP] {P : PROP} (A : Atom PROP α) (a : α) (E : Unit → PROP)
+  (_h : P ∗ A # a ⊢ E ())
+ : P ⊢ (inhaleR (atom_with_ref A a)) E := by
+    simp [inhaleR, atom_with_ref]
+    mysorry
+
+@[irun_tac (inhaleR (atom_with_ref _ _)) _]
+def irunInhaleAtomWithRef : IRunTacticType := fun goal _config => do profileitM Exception "irunInhaleAtomWithRef" (← getOptions) do
+  let { u, prop, bi, hyp, goal:=G } := goal
+  let_expr inhaleR _ _ _ L E := G | return none
+  let_expr atom_with_ref _ α A a := L | return none
+  let .some ⟨e, hyps⟩ := parseHypsFromShallow? u prop bi hyp | return none
+  let us := L.getAppFn'.constLevels!
+  let ident ← `(binderIdent| _)
+  let goals ← IO.mkRef #[]
+  let Q := Expr.beta E #[mkConst ``Unit.unit]
+  let A' := mkApp4 (.const ``Atom.ref us) prop α A a
+  let pf ← iCasesCore bi hyps Q q(false) A' A' ⟨⟩ (.one ident) fun hyps => do
+    let m ← mkFreshExprSyntheticOpaqueMVar <|
+      IrisGoal.toExpr { u, prop, bi, e:=_, hyps, goal:=Q }
+    goals.modify (·.push m.mvarId!)
+    return m
+  let pf := mkApp8 (.const ``inhale_atom_with_ref_tac us) prop α bi e A a E pf
+  return .some (pf, (← goals.get).toList, [])
+
+theorem inhale_pers_atom_with_ref_tac {α : Type _} [BI PROP] {P : PROP} (A : Atom PROP α) (a : α) (E : Unit → PROP)
+  (_h : P ∗ □ A # a ⊢ E ())
+ : P ⊢ (inhaleR (pers (atom_with_ref A a))) E := by
+    simp [inhaleR, atom_with_ref]
+    mysorry
+
+-- TODO: unify with irunInhaleAtomWithRef?
+@[irun_tac (inhaleR (pers (atom_with_ref _ _))) _]
+def irunInhalePersAtomWithRef : IRunTacticType := fun goal _config => do profileitM Exception "irunInhaleAtomWithRef" (← getOptions) do
+  let { u, prop, bi, hyp, goal:=G } := goal
+  let_expr inhaleR _ _ _ L E := G | return none
+  let_expr pers _ _ _ L := L | return none
+  let_expr atom_with_ref _ α A a := L | return none
+  let .some ⟨e, hyps⟩ := parseHypsFromShallow? u prop bi hyp | return none
+  let us := L.getAppFn'.constLevels!
+  let ident ← `(binderIdent| _)
+  let goals ← IO.mkRef #[]
+  let Q := Expr.beta E #[mkConst ``Unit.unit]
+  let A' := mkApp4 (.const ``Atom.ref us) prop α A a
+  let A'' := mkApp3 (.const ``intuitionistically [u]) prop (mkApp2 (.const ``BI.toBIBase [u]) prop bi) A'
+  let pf ← iCasesCore bi hyps Q q(true) A'' A' ⟨⟩ (.one ident) fun hyps => do
+    let m ← mkFreshExprSyntheticOpaqueMVar <|
+      IrisGoal.toExpr { u, prop, bi, e:=_, hyps, goal:=Q }
+    goals.modify (·.push m.mvarId!)
+    return m
+  let pf := mkApp8 (.const ``inhale_pers_atom_with_ref_tac us) prop α bi e A a E pf
+  return .some (pf, (← goals.get).toList, [])
+
+theorem inhale_prop_tac [BI PROP] φ (P : PROP) E
+  (_h : φ → P ⊢ E ())
+ : P ⊢ inhaleR (prop φ) E := by
+   mysorry
+
+
+-- TODO: There are really strange compiler bugs here. If this
+-- definition is inline, lean crashes in files that import this one
+-- and use irunInhaleProp. Using [noinline] does not help. Also
+-- removing irunInhaleProp2, which is unused, causes the crash
+def irunInhalePropCases (m : MVarId) (n : Name) : TacticM (List MVarId) :=
+  m.withContext do
+    let some d := (← getLCtx).findFromUserName? n | throwError "cannot find freshly generated name"
+    let ty := d.type
+    -- TODO: when to we want to call cases?
+    unless ty.isEq || ty.isFalse || ty.isTrue do
+      return [m]
+    let r? ← observing? (m.cases d.fvarId)
+    return r?.elim [m] (λ m => m.toList.map (·.mvarId))
+
+def irunInhaleProp2 : IRunTacticType := fun goal _config => do profileitM Exception "irunInhaleProp" (← getOptions) do
+  let { u, prop, bi, hyp, goal:=G } := goal
+  let_expr inhaleR _ _ _ L E := G | return none
+  let_expr prop _ _ φ := L | return none
+  let n ← mkFreshUserName (.mkStr1 "h")
+  let (pf, m) ← withLocalDeclD n φ fun x => do
+    -- TODO: iintros has this, what does this do?
+    -- addLocalVarInfo ref (← getLCtx) x α
+    let m ← mkFreshExprSyntheticOpaqueMVar <|
+        IrisGoalShallow.toExpr { u, prop, bi, hyp, goal := Expr.beta E #[mkConst ``Unit.unit]}
+    let mbound ← mkLambdaFVars #[x] m
+    let pf := mkApp6 (.const ``inhale_prop_tac [u]) prop bi φ hyp E mbound
+    return (pf, m.mvarId!)
+  let mvars ← irunInhalePropCases m n
+  --let mvars := [m]
+  return .some (pf, mvars, [])
+
+
+@[irun_tac inhaleR (prop _) _]
+def irunInhaleProp : IRunTacticType := fun goal _config => do profileitM Exception "irunInhaleProp" (← getOptions) do
+  let { u, prop, bi, hyp, goal:=G } := goal
+  let_expr inhaleR _ _ _ L E := G | return none
+  let_expr prop _ _ φ := L | return none
+  let n ← mkFreshUserName (.mkStr1 "h")
+  let (pf, m) ← withLocalDeclD n φ fun x => do
+    -- TODO: iintros has this, what does this do?
+    -- addLocalVarInfo ref (← getLCtx) x α
+    let m ← mkFreshExprSyntheticOpaqueMVar <|
+        IrisGoalShallow.toExpr { u, prop, bi, hyp, goal := Expr.beta E #[mkConst ``Unit.unit]}
+    let mbound ← mkLambdaFVars #[x] m
+    let pf := mkApp6 (.const ``inhale_prop_tac [u]) prop bi φ hyp E mbound
+    return (pf, m.mvarId!)
+  let tac ← `(tactic|simp [*, irun_simp] at $(mkIdent n):ident)
+  let res ← try
+      evalTacticAtRaw tac m
+    catch _e =>
+      --logInfo m!"{e.toMessageData}"
+      .pure [m]
+  if res == [] then return .some (pf, [], [])
+  let [m] := res | throwError "simp created too many subgoals"
+  let mvars ← irunInhalePropCases m n
+  return .some (pf, mvars, [])
+
+end inhale
+
+section exhale
+
+@[irun]
+theorem cancel_match [BI PROP] {α : Type _} (A : Atom PROP α) a E :
+  cancelR (A # a) A E ⊣ E a := by mysorry
+
+@[irun]
+theorem exhaleR_persLi (α : Type _) [BI PROP] (G : Li PROP α) :
+  exhaleR (PROP:=PROP) (persLi G) :-
+    branch ((dropSpatial G).bind λ _ => Lithium.done) (return ()) := by
+  mysorry
+
+@[irun]
+theorem exhale_atom_with_ref [BI PROP] {α : Type _} (A : Atom PROP α) a (E : Unit → PROP) :
+   exhaleR (atom_with_ref A a) E ⊣ exhaleR (atom A) λ a' => exhaleR (prop (a = a')) λ _ => E () :=
+   by mysorry
+
+@[irun]
+theorem exhale_prop [BI PROP] P (E : Unit → PROP) :
+   P →
+   exhaleR (prop P) E ⊣ E () :=
+   by mysorry
+
+
+theorem exhale_atom_direct_tac {α : Type _} [BI PROP] {p : Bool} {P P' : PROP} (A : Atom PROP α) (a : α) {E}
+  (_hP : P ⊣⊢ P' ∗ □?p A # a)
+  (_h : P' ⊢ E a)
+ : P ⊢ exhaleR (atom A) E := by
+   mysorry
+
+@[irun_tac exhaleR (atom _) _]
+def irunExhaleAtomDirect : IRunTacticType := fun goal _config => do profileitM Exception "irunExhaleAtomDirect" (← getOptions) do
+  let {u, prop, bi, hyp, goal:=G} := goal
+  let_expr exhaleR _ _ _ L E := G | return none
+  let_expr atom _ α A := L | return none
+  let .some ⟨e, hyps⟩ := parseHypsFromShallow? u prop bi hyp | return none
+  let us := L.getAppFn'.constLevels!
+  let some ⟨a, P', hyps, _out, _ty, b, _, pf⟩ ←
+    hyps.removeG false fun _ _ _ ty => do
+      let_expr Atom.ref _ _ A' a := ty | return none
+      let eq ← withReducible <| isDefEq A' A
+      -- logInfo m!"ty: {ty}, A: {A} / {repr A}, A': {A'} / {repr A'}, eq: {eq}"
+      if eq then return some a else return none
+    | return none
+  let m ← mkFreshExprSyntheticOpaqueMVar <|
+    IrisGoal.toExpr { u, prop, bi, e:=_, hyps := hyps, goal := Expr.beta E #[a] }
+  let pf := mkApp11 (.const ``exhale_atom_direct_tac us) prop α bi b e P' A a E pf m
+  return .some (pf, [m.mvarId!], [])
+
+theorem exhale_atom_cancel_tac {α : Type _} [BI PROP] {p : Bool} {P P' Q : PROP} (A : Atom PROP α) {E}
+  (_hP : P ⊣⊢ P' ∗ □?p Q)
+  (_h : P' ⊢ cancelR Q A E)
+ : P ⊢ exhaleR (atom A) E := by
+   mysorry
+
+-- below default priority for direct cancelation since direct cancellation can be a lot faster
+@[irun_tac:mid exhaleR (atom _) _]
+def irunExhaleAtomCancel : IRunTacticType := fun goal config => do profileitM Exception "irunExhaleAtomCancel" (← getOptions) do
+  let { u, prop, bi, hyp, goal:=G } := goal
+  let_expr exhaleR _ _ _ L E := G | return none
+  let_expr atom _ α A := L | return none
+  let .some ⟨e, hyps⟩ := parseHypsFromShallow? u prop bi hyp | return none
+  let hyp' := ← mkFreshExprMVar (.some prop)
+  let us := L.getAppFn'.constLevels!
+  let tree := irunExt.getState (← getEnv)
+  let some ⟨(tacpf, goals, shelved), P', hyps, _out, ty, b, _, pf⟩ ←
+    hyps.removeG false fun _ _ _ Q => do
+      let ig' := { u, prop, bi, hyp := hyp', goal := mkApp6 (.const ``cancelR us) prop bi α Q A E }
+      let .some (pf, goals, shelved) ← irunSearch config ig' tree | return none
+      return (pf, goals, shelved)
+    | return none
+  hyp'.mvarId!.assign hyps.tm
+  let pf := mkApp11 (.const ``exhale_atom_cancel_tac us) prop α bi b e P' ty A E pf tacpf
+  return .some (pf, goals, shelved)
+
+
+theorem exhale_prop_tac [BI PROP] (P : PROP) (φ : Prop) E
+  (_hφ : φ)
+  (_h : P ⊢ E ())
+ : P ⊢ exhaleR (prop φ) E := by
+   mysorry
+
+@[irun_tac:low exhaleR (prop _) _]
+def irunExhaleProp : IRunTacticType := fun goal _config => do profileitM Exception "irunExhaleProp" (← getOptions) do
+  let { u, prop, bi, hyp, goal:=G } := goal
+  let_expr exhaleR _ _ _ L E := G | return none
+  let_expr prop _ _ P := L | return none
+  let mP ← mkFreshExprSyntheticOpaqueMVar P
+  let m ← mkFreshExprSyntheticOpaqueMVar <|
+      IrisGoalShallow.toExpr { u, prop, bi, hyp, goal := Expr.beta E #[mkConst ``Unit.unit] }
+  let pf := mkApp7 (.const ``exhale_prop_tac [u]) prop bi hyp P E mP m
+  return .some (pf, [m.mvarId!], [mP.mvarId!])
+
+end exhale
+
+section all
+
+theorem all_tac [BI PROP] {α : Type _} (P : PROP) E
+  (_h : ∀ a : α, P ⊢ E a)
+ : P ⊢ allR E := by
+   mysorry
+
+@[irun_tac allR _]
+def irunAll : IRunTacticType := fun goal _config => do profileitM Exception "irunAll" (← getOptions) do
+  let { u, prop, bi, hyp, goal:=G } := goal
+  let_expr allR _ _ α E := G | return none
+  -- TODO: can we generate better names?
+  let n ← mkFreshUserName (.mkStr1 "x")
+  let (pf, m) ← withLocalDeclD n α fun x => do
+    -- addLocalVarInfo ref (← getLCtx) x α
+    let m ← mkFreshExprSyntheticOpaqueMVar <|
+      IrisGoalShallow.toExpr { u, prop, bi, hyp, goal := Expr.beta E #[x] }
+    let mbound ← mkLambdaFVars #[x] m
+    let pf := mkApp6 (.const ``all_tac G.getAppFn'.constLevels!) prop bi α hyp E mbound
+    return (pf, m)
+  return .some (pf, [m.mvarId!], [])
+
+end all
+
+section done
+theorem done_tac [BI PROP] (P : PROP)
+ : P ⊢ doneR := pure_intro .intro
+
+@[irun_tac doneR]
+def irunDone : IRunTacticType := fun goal _config => do profileitM Exception "irunDone" (← getOptions) do
+  let { u:=_, prop, bi, hyp, goal:=G } := goal
+  let .true := G.isAppOfArity ``doneR 2 | return none
+  let pf := mkApp3 (.const ``done_tac G.getAppFn'.constLevels!) prop bi hyp
+  return .some (pf, [], [])
+
+end done
+
+section branch
+@[irun]
+theorem lif_true [BI PROP] {cond : Prop} (E1 E2 : PROP) :
+   cond →
+   lifR cond E1 E2 ⊣ E1  :=
+   by mysorry
+
+@[irun]
+theorem lif_false [BI PROP] {cond : Prop} (E1 E2 : PROP) :
+   ¬ cond →
+   lifR cond E1 E2 ⊣ E2 :=
+   by mysorry
+
+@[irun:low]
+theorem lif_branch [BI PROP] {cond : Prop} (E1 E2 : PROP) :
+   lifR cond E1 E2 ⊣ branchR (inhaleR (prop cond) λ _ => E1) (inhaleR (prop (¬ cond)) λ _ => E2) :=
+   by mysorry
+
+theorem branch_tac [BI PROP] P (E1 E2 : PROP)
+  (_ : P ⊢ E1)
+  (_ : P ⊢ E2)
+ : P ⊢ branchR E1 E2 := by
+   simp [branchR]
+   apply and_intro <;> trivial
+
+
+@[irun_tac branchR _ _]
+def irunBranch : IRunTacticType := fun goal _config => do profileitM Exception "irunBranch" (← getOptions) do
+  let ig := goal
+  let { u, prop, bi, hyp, goal:=G } := ig
+
+  let_expr branchR _ _ E1 E2 := G | return none
+  let m1 ← mkFreshExprSyntheticOpaqueMVar <| IrisGoalShallow.toExpr { ig with goal := E1 }
+  let m2 ← mkFreshExprSyntheticOpaqueMVar <| IrisGoalShallow.toExpr { ig with goal := E2 }
+  let pf := mkApp7 (.const ``branch_tac [u]) prop bi hyp E1 E2 m1 m2
+  return .some (pf, [m1.mvarId!, m2.mvarId!], [])
+
+end branch
+
+section dropSpatial
+
+theorem drop_spatial_tac [BI PROP] [BIAffine PROP] P Ps Pi (E : PROP)
+  (_ : P ⊣⊢ Ps ∗ □ Pi)
+  (_ : Pi ⊢ E)
+ : P ⊢ dropSpatialR E := by
+    mysorry
+
+@[irun_tac dropSpatialR _]
+def irunDropSpatial : IRunTacticType := fun goal _config => do profileitM Exception "irunDropSpatial" (← getOptions) do
+  let { u, prop, bi, hyp, goal:=G } := goal
+  let_expr dropSpatialR _ _ E := G | return none
+  let .some ⟨e, hyps⟩ := parseHypsFromShallow? u prop bi hyp | return none
+  let .some aff ← synthInstance? (mkApp2 (.const ``BIAffine [u]) prop bi) | throwError "cannot synthesize BIAffine"
+  let ⟨es, _, ei, hypsi, pf⟩ := hyps.partition
+  let m ← mkFreshExprSyntheticOpaqueMVar <|
+    IrisGoalShallow.toExpr { u, prop, bi, hyp := hypsi.tm, goal := E }
+  let pf := mkApp9 (.const ``drop_spatial_tac [u]) prop bi aff e es ei E pf m
+  return .some (pf, [m.mvarId!], [])
+
+end dropSpatial
+
+section simp
+
+@[irun_tac simpR _ _ _ _]
+def irunSimp : IRunTacticType := fun goal _config => do profileitM Exception "irunSimp" (← getOptions) do
+  let ig := goal
+  let G := ig.goal
+
+  let_expr simpR _ _ _ n dodsimp e E := G | return none
+  let n : Name ← reduceEval n
+  let dodsimp : Bool ← reduceEval dodsimp
+  if dodsimp then
+    let ⟨e_new, _⟩ ← dsimpWithExt n e
+    let g' := {ig with goal := Expr.beta E #[e_new]}.toExpr
+    let goal' ← mkFreshExprSyntheticOpaqueMVar g'
+    let pf ← mkExpectedTypeHint goal' ig.toExpr
+    return .some (pf, [goal'.mvarId!], [])
+  else
+    throwError "simp not implemented"
+
+end simp
+
+section dualizing
+
+@[irun]
+theorem dualizing_exhale [BI PROP] α (L : InEx PROP α) (G : (Empty → PROP) → α → PROP) E :
+  dualizingR (PROP:=PROP) (λ E => exhaleR L (G E)) E ⊣
+   inhaleR L λ a =>
+   dualizingR (λ E => G E a) E := by mysorry
+
+@[irun]
+theorem dualizing_inhale [BI PROP] α (L : InEx PROP α) (G : (Empty → PROP) → α → PROP) E :
+  dualizingR (PROP:=PROP) (λ E => inhaleR L (G E)) E ⊣
+   exhaleR L λ a =>
+   dualizingR (λ E => G E a) E := by mysorry
+
+@[irun]
+theorem dualizing_done [BI PROP] E :
+  dualizingR (PROP:=PROP) (λ _ => doneR) E ⊣ E () := by mysorry
+end dualizing
+
+section test
+variable [BI.{u} PROP]
+
+example (P : Nat → Atom PROP Unit) (Q : Atom PROP Unit) :
+  ⊢ (do
+      inhale (PROP:=PROP) (atom_with_ref Q ())
+      let n ← all
+      let m ← all
+      inhale (atom_with_ref (P n) ())
+      inhale (atom_with_ref (P m) ())
+      inhale (atom_with_ref (P 1) ())
+      exhale do
+        atom (P n)
+        atom (P m)
+        atom (P 1)
+      exhale (atom Q)
+      done).go := by
+     istart
+     simp only [irun_preprocess]
+     irun
+
+example (P G : Atom PROP Unit) :
+  ⊢ (do
+      inhale (PROP := PROP) do
+        atom_with_ref P ()
+        atom_with_ref G ()
+      exhale do
+        atom G
+      done).go := by
+    istart
+    simp only [irun_preprocess]
+    irun
+
+/-
+not reversed:
+- time with direct cancellation for 100: 659ms
+- time with direct cancellation for 200: 2873ms
+- time with generic cancellation for 100: 1461ms (when creating mvars: 10884ms)
+- time with generic cancellation for 200: 5782ms (when creating mvars: 39206ms)
+reversed:
+- time is basically identical between the two versions
+-/
+--set_option profiler true in
+--set_option profiler.threshold 1 in
+set_option maxRecDepth 30000 in
+set_option maxHeartbeats 2000000 in
+set_option Elab.async false in
+-- set_option trace.profiler true in
+-- set_option trace.IRun.step true in
+#time example (P : Nat → Atom PROP Unit) :
+  ⊢ inhaleR (List.foldl (λ G n => ((atom_with_ref (P n) ()).bind λ _ => G)) (.pure tt) (List.range 100)) λ _ =>
+    (List.foldl (λ G n => exhaleR (atom (P n)) λ _ => G)
+      (doneR) (
+    -- List.reverse makes cancellation faster
+    -- List.reverse
+    (List.range 100)))
+
+:=
+  by
+    dsimp [List.foldl, List.range, List.range.loop, List.reverse]
+    istart
+    irun
+
+end test
+
+end Iris.Lithium
