src/Iris/Lithium/Time.lean
@@ -1,0 +1,23 @@
+import Iris.BI
+import Iris.ProofMode
+import Iris.Lithium.IRunAttr
+import Iris.Lithium.IRun
+import Iris.Lithium.Exp
+import Iris.Lithium.Lithium
+import Iris.Lithium.ExpLi
+
+namespace Iris.ExampleLang
+open BI
+
+variable [BI PROP]
+
+set_option Elab.async false in
+example [BI PROP] [BIAffine PROP] P :
+  ⊢ contains_spec (PROP:=PROP) P := by
+  unfold contains_spec contains_spec_pre contains_spec_post contains_fn
+  apply (BI.BIBase.Entails.trans _ (prove_fn_spec _ _ _))
+  istart
+  simp only [irun_preprocess]
+  irun
+  rename List Val => xs
+  cases xs <;> simp at *
